incomplete proofs of helper functions in HBRaceDetector

HBRaceDetector.v
@@ -21,16 +21,27 @@ Proof.
   unfold upd_env, upd; clarify.
 Qed.
 
+Lemma upd_overwrite : forall G t a v1 v2,
+  upd_env (upd_env G t a v1) t a v2 = upd_env G t a v2.
+Proof.
+  Admitted.
+
+
+Definition events_move (src tgt:ptr) (t:tid): list Lang.operation := [rd t src; wr t tgt].
+
+Definition mops_move (src tgt: ptr) (t:tid) (v:nat): list conc_op := [Read t src v; Write t tgt v].
+
 Lemma move_spec : forall src tgt tmp P P1 P2 G t rest v
   (Hmove : P = P1 ++ (t, move src tgt tmp ++ rest) :: P2),
   exec_star (Some P) G
-            [rd t src; wr t tgt] [Read t src v; Write t tgt v]
+            (events_move src tgt t) (mops_move src tgt t v)
     (Some (P1 ++ (t, rest) :: P2)) (upd_env G t tmp v).
 Proof.
-  intros.
+    
+  intros. 
   eapply exec_step'.
   - apply exec_load.
-    unfold move in Hmove; eauto.
+    unfold move in Hmove.  eauto.
   - simpl.
     eapply exec_step'.
     + apply exec_store.
@@ -49,9 +60,53 @@ Fixpoint set_vc (tgt : var (* loc of target VC *))
   (tmp : local (* a local to use as temp *)) :=
 (* Move all z of the timestamps in src into tgt. *)
 match z with
-| O => []
-| S n => move (src, n) (tgt, n) tmp ++ set_vc tgt src n tmp
+| 0 => []
+| S n =>  move (src,n) (tgt,n) tmp++set_vc tgt src n tmp 
 end.
+
+Fixpoint events_set_vc (src tgt: var) (z : nat) (t : tid) : list Lang.operation:=
+match z with
+| O => []
+| S n => (events_move (src,n) (tgt,n) t)++events_set_vc src tgt n t
+end.
+
+Fixpoint mops_set_vc (src tgt: var) (z : nat) (t : tid) (vs: list nat): list conc_op :=
+match (z,vs) with
+| (S n,v::vss) => (mops_move (src,n) (tgt,n) t v)++mops_set_vc src tgt n t vss
+| _ => []
+end.
+
+Lemma empty_list : forall (vs:list nat) (Hl: (length vs) = 0), vs=[]. 
+Admitted.
+
+Lemma set_vc_spec_0 : forall tgt src tmp P G P1 P2 t rest 
+(Hset_vc0: P=P1++(t, set_vc tgt src 0 tmp ++ rest)::P2),
+exec_star (Some P) G [] [] (Some (P1++(t,rest)::P2)) G.
+Proof.
+  intros.
+  unfold set_vc in Hset_vc0.
+  rewrite Hset_vc0.
+  simpl.
+  eapply exec_refl.
+Qed.
+
+
+Lemma set_vc_spec_n : forall tgt src n tmp P G P1 P2 t rest v vss 
+(Hset_vc: P=P1++(t, set_vc tgt src (S n) tmp++ rest)::P2) (Hvs: length vss=n),
+ exec_star (Some P) G
+          (events_set_vc src tgt (S n) t) (mops_set_vc src tgt (S n) t (vss++[v])) (Some (P1++(t,rest)::P2)) (upd_env G t tmp v).
+Proof.
+  
+  intros.
+  induction n.
+
+  -apply empty_list in Hvs.
+   clarify.
+   apply move_spec.
+   eauto.
+  -Abort.
+  
+ 
 
 Definition inc_vc t tgt tmp := [
   Load tmp (tgt, t);
@@ -59,26 +114,147 @@ Definition inc_vc t tgt tmp := [
   Store (tgt, t) (V tmp)
 ].
 
+Definition events_inc_vc (tgt:var) (t:tid): list Lang.operation:=
+  [rd t (tgt,t); wr t (tgt,t)]. 
+Definition mops_inc_vc (tgt:var) (v:nat) (t:tid): list conc_op:=
+  [Read t (tgt,t) v; Write t (tgt,t) (v+1) ].
+
+Lemma inc_vc_spec : forall  tgt tmp P G P1 P2 t rest v 
+  (Hinc_vc: P=P1++((t,inc_vc t tgt tmp++rest)::P2)),
+  exec_star (Some P) G 
+            (events_inc_vc tgt t) (mops_inc_vc tgt v t) 
+            (Some (P1++(t,rest)::P2)) (upd_env G t tmp (v+1)). 
+Proof.
+  intros.
+  eapply exec_step'.
+  -apply exec_load.
+   unfold inc_vc in Hinc_vc; eauto.
+  -simpl.
+   eapply exec_step'.
+   +apply exec_assign; eauto.
+   +simpl.
+    
+    eapply exec_step'.
+    *apply exec_store; eauto.
+    *rewrite upd_same.
+     rewrite upd_overwrite.
+     apply exec_refl.
+    *auto.
+    *auto.
+   +auto.
+   +auto.
+  -auto.
+  -simpl.
+   unfold mops_inc_vc.
+   repeat rewrite upd_same.
+   auto.
+Qed.
+
+Fixpoint max tgt src tmp1 tmp2 :=
+[
+  Load tmp1 src;
+  Load tmp2 tgt;
+  Assign tmp2 (Max (V tmp1) (V tmp2));
+  Store tgt (V tmp2)
+].
+
+Definition events_max (src tgt:ptr) (t:tid) : list Lang.operation :=
+[
+  rd t src ;
+  rd t tgt ;
+  wr t tgt
+]. 
+
+Definition mops_max (src tgt: ptr) (v1 v2 : nat) (t:tid): list conc_op:=
+[
+  Read t src v1;
+  Read t tgt v2
+  (*;Write t tgt (nat.max v1 v2)*)
+].
+
 Fixpoint max_vc tgt src z tmp1 tmp2 :=
 match z with
 | 0 => []
-| S n => [
-    Load tmp1 (src,n); 
-    Load tmp2 (tgt,n);
-    Assign tmp2 (Max (V tmp1) (V tmp2));
-    Store (tgt,n) (V tmp2)
-]++ max_vc tgt src n tmp1 tmp2
+| S n => max (tgt,n) (src,n) tmp1 tmp2++ max_vc tgt src n tmp1 tmp2
 end.
+
+Fixpoint events_max_vc (src tgt:var) (t: tid) (z:nat): list Lang.operation:=
+match z with
+|0 => []
+|S n => events_max (src,n) (tgt,n) t ++ events_max_vc src tgt t n
+end.
+
+Fixpoint mops_max_vc (src tgt: var) (vs1 vs2: list nat) (t:tid) (z:nat) : list conc_op:=
+match (z,vs1,vs2) with
+|(0,[],[]) => []
+|(S n,v1::vss1,v2::vss2) => mops_max (src,n) (tgt,n) v1 v2 t ++ mops_max_vc src tgt vss1 vss2 t z 
+| _ => []
+end. 
+Lemma max_vc_spec_0 : forall src tgt tmp1 tmp2 P G P1 P2 t rest
+(Hmax_vc0 : P=P1++(t, max_vc src tgt 0 tmp1 tmp2 ++ rest)::P2),
+ exec_star (Some P) G 
+           [] [] (Some (P1++(t,rest)::P2)) G.
+Proof.
+  intros.
+  unfold max_vc in Hmax_vc0.
+  rewrite Hmax_vc0.
+  eapply exec_refl.
+Qed.
+
+Lemma max_vc_spec_n : forall src tgt n tmp1 tmp2 P G P1 P2 t rest v1 v2 vss1 vss2
+
+(Hmax_vc: P=P1++(t, max_vc src tgt (S n) tmp1 tmp2 ++ rest)::P2) (Hvs1: length vss1=n) (Hvs2: length vss2=n),
+ exec_star (Some P) G
+          (events_max_vc src tgt t (S n)) (mops_max_vc src tgt (vss1++[v1]) (vss2++[v2]) t (S n)) (Some (P1++(t,rest)::P2)) (upd_env (upd_env G t tmp1 v1) t tmp2 v2).
+  
+Definition assert_le (a b : ptr) (tmp1 tmp2:local): prog :=
+[
+    Load tmp1 a;
+    Load tmp2 b;
+    Assert_le (V tmp1) (V tmp2)
+].
+
+Definition events_assert_le (a b: ptr) (t:tid) : list Lang.operation :=
+[
+  rd t a;
+  rd t b
+].
+
+Definition mops_assert_le (a b : ptr) (v1 v2: nat) (t: tid): list conc_op :=
+[
+  Read t a v1;
+  Read t b v2
+].
+
 
 Fixpoint hb_check C1 C2 z tmp1 tmp2 :=
 match z with
 | 0 => []
-| S n => [
-    Load tmp1 (C1, n);
-    Load tmp2 (C2, n);
-    Assert_le (V tmp1) (V tmp2)
-]++ hb_check C1 C2 n tmp1 tmp2
+| S n =>(assert_le (C1,n) (C2,n) tmp1 tmp2)++ hb_check C1 C2 n tmp1 tmp2
 end.
+
+Fixpoint events_hb_check (C1 C2: var) (z:nat) (t:tid) : list Lang.operation :=
+match z with
+| 0 => []
+| S n => events_assert_le (C1,n) (C2,n) t++events_hb_check C1 C2 n t
+end.
+
+Fixpoint mops_hb_check (C1 C2: var) (vs1 vs2: list nat) (z:nat) (t:tid) : list conc_op :=
+match (z,vs1,vs2) with
+| (S n, v1::vss1, v2::vss2) => mops_assert_le (C1,n) (C2,n) v1 v2 t ++ mops_hb_check C1 C2 vss1 vss2 n t
+| _ => []
+end.
+
+Lemma hb_check_spec0: forall C1 C2 t tmp1 tmp2 P G P1 P2 rest
+ (Hhb_check0: P=P1++(t,hb_check C1 C2 0 tmp1 tmp2++rest)::P2),
+  exec_star (Some P) G 
+            [] [] (Some (P1++(t,rest)::P2)) G.
+Proof.
+  intros.
+  unfold hb_check in Hhb_check0; eauto.
+  rewrite Hhb_check0.
+  apply exec_refl.
+Qed.
 
 (* Since everything is a nat, we can use C + t as the t component of C. *)
 Definition load_handler t x C R (W : var) z tmp1 tmp2 := 
